Simpler proof idea from Steven (blocked on #195)

examples/metatheory/stlc_strong_db_parsubst.fst
@@ -259,6 +259,23 @@ let rec substitution_preserves_typing x e v t_x t g h1 h2 =
     (TyApp (substitution_preserves_typing x h1 h21)
            (substitution_preserves_typing x h1 h22))
 
+(* Simpler proof idea from Steven (blocked on #195)
+
+(*
+type subst_typing (s:sub) (g1:env) (g2:env) =
+  (forall (x:var). is_Some (g1 x) ==> typing g2 (s x) (Some.v (g1 x)))
+*)
+type subst_typing (s:sub) (g1:env) (g2:env) =
+  (x:var{is_Some (g1 x)} -> typing g2 (s x) (Some.v (g1 x)))
+
+val substitution :
+      #g1:env -> #e:exp -> #t:typ -> #s:sub -> #g2:env ->
+      h1:typing g1 e t ->
+      hs:subst_typing s g1 g2 ->
+      Tot (typing g2 (subst s e) t) (decreases e)
+let substitution g1 e t s g2 h1 hs = magic()
+*)
+
 (* Type preservation *)
 
 opaque val preservation : #e:exp -> #e':exp -> hs:step e e' ->
